New proof of alloc_disjoint in infinite / finite setting.

src/rocq/Utils/CTreeMemExample.v
@@ -12,6 +12,7 @@ From Stdlib Require Import
   Lia.
 
 Module IM := FMapAVL.Make(Stdlib.Structures.OrderedTypeEx.Z_as_OT).
+Module Import IP := FMapFacts.WProperties_fun(Stdlib.Structures.OrderedTypeEx.Z_as_OT)(IM).
 
 (* (* For some reason this causes universe inconsistencies *) *)
 (* From Vellvm Require Import *)
@@ -42,54 +43,55 @@ From Stdlib Require Import ZArith String.
 
 Import CTreeNotations.
 
-(* Memory that's just an IntMap of possibly allocated nat "bytes" *)
-Definition memory := IM.t nat.
-Definition memory_size : option Z := Some 10%Z.
+Section Memory.
+  (* Memory that's just an IntMap of possibly allocated nat "bytes" *)
+  Definition memory := IM.t nat.
+  Variable (memory_size : option N).
 
-Variant MemE : Type -> Type :=
-  | LoadE (key : Z) : MemE nat
-  | StoreE (key : Z) (val : nat) : MemE unit
-  | AllocE : MemE Z.
+  Variant MemE : Type -> Type :=
+    | LoadE (key : Z) : MemE nat
+    | StoreE (key : Z) (val : nat) : MemE unit
+    | AllocE : MemE Z.
 
-(* Failure. Carries a string for a message. *)
-Variant FailureE : Type -> Type :=
-  | Throw : unit -> FailureE void.
+  (* Failure. Carries a string for a message. *)
+  Variant FailureE : Type -> Type :=
+    | Throw : unit -> FailureE void.
 
-(* This function can be replaced with print_string during extraction
+  (* This function can be replaced with print_string during extraction
      to print the error messages of Throw and (indirectly) ThrowUB. *)
-Definition print_msg (msg : string) : unit := tt.
+  Definition print_msg (msg : string) : unit := tt.
 
-Definition raise {E B} {A} `{FailureE -< E} (msg : string) : ctree E B A :=
-  v <- trigger (Throw (print_msg msg));; match v: void with end.
+  Definition raise {E B} {A} `{FailureE -< E} (msg : string) : ctree E B A :=
+    v <- trigger (Throw (print_msg msg));; match v: void with end.
 
-(* Out of memory / abort. Carries a string for a message. *)
-Variant OOME : Type -> Type :=
-  | ThrowOOM : unit -> OOME void.
+  (* Out of memory / abort. Carries a string for a message. *)
+  Variant OOME : Type -> Type :=
+    | ThrowOOM : unit -> OOME void.
 
-(** Since the output type of [ThrowUB] is [void], we can make it an action
+  (** Since the output type of [ThrowUB] is [void], we can make it an action
     with any return type. *)
-Definition raiseOOM {E : Type -> Type} {BR} {X} `{OOME -< E}
-  (e : string)
-  : ctree E BR X
-  := v <- trigger (ThrowOOM (print_msg e));; match v: void with end.
+  Definition raiseOOM {E : Type -> Type} {BR} {X} `{OOME -< E}
+    (e : string)
+    : ctree E BR X
+    := v <- trigger (ThrowOOM (print_msg e));; match v: void with end.
 
-Fixpoint IM_raw_greatest_key {A} (m : IM.Raw.tree A) : option Z
-  := match m with
-     | IM.Raw.Leaf _ => None
-     | IM.Raw.Node l k _ (@IM.Raw.Leaf _) _ =>
-         ret k
-     | IM.Raw.Node l k _ r _ =>
-         IM_raw_greatest_key r
-     end.
+  Fixpoint IM_raw_greatest_key {A} (m : IM.Raw.tree A) : option Z
+    := match m with
+       | IM.Raw.Leaf _ => None
+       | IM.Raw.Node l k _ (@IM.Raw.Leaf _) _ =>
+           ret k
+       | IM.Raw.Node l k _ r _ =>
+           IM_raw_greatest_key r
+       end.
 
-Definition IM_greatest_key {A} (m : IM.t A) : option Z
-  := IM_raw_greatest_key (IM.this m).
+  Definition IM_greatest_key {A} (m : IM.t A) : option Z
+    := IM_raw_greatest_key (IM.this m).
 
-Definition next_key {A} (m : IM.t A) : Z
-  := match IM_greatest_key m with
-     | Some k => 1 + k
-     | None => 0
-     end.
+  Definition next_key {A} (m : IM.t A) : Z
+    := match IM_greatest_key m with
+       | Some k => 1 + k
+       | None => 0
+       end.
 
   Lemma IM_greatest_key_none' :
     forall {A} (m : IM.t A), IM.Empty m -> IM_greatest_key m = None.
@@ -302,77 +304,88 @@ Definition next_key {A} (m : IM.t A) : Z
   Qed.
 
 
-Definition handle_mem {E} `{FailureE -< E} `{OOME -< E} : MemE ~> Monads.stateT memory (ctree E void1) :=
-  fun _ e mem =>
-    match e with
-    | LoadE k =>
-        match IM.find k mem with
-        | Some v => ret (mem, v)
-        | None => raise "Load from unallocated address."
-        end
-    | StoreE k v =>
-        match IM.find k mem with
-        | Some _ =>
-            let mem' := IM.add k v mem in
-            ret (mem', tt)
-        | None => raise "Store to unallocated address."
-        end
-    | AllocE =>
-        let k := next_key mem in
-        match memory_size with
-        | Some sz =>
-            if (k <=? sz)%Z
-            then ret (IM.add k 0 mem, k)
-            else raiseOOM "Not enough memory."
-        | None => ret (IM.add k 0 mem, k)
-        end
+  Definition handle_mem {E} `{FailureE -< E} `{OOME -< E} : MemE ~> Monads.stateT memory (ctree E void1) :=
+    fun _ e mem =>
+      match e with
+      | LoadE k =>
+          match IM.find k mem with
+          | Some v => ret (mem, v)
+          | None => raise "Load from unallocated address."
+          end
+      | StoreE k v =>
+          match IM.find k mem with
+          | Some _ =>
+              let mem' := IM.add k v mem in
+              ret (mem', tt)
+          | None => raise "Store to unallocated address."
+          end
+      | AllocE =>
+          let k := next_key mem in
+          match memory_size with
+          | Some sz =>
+              if (k <=? Z.of_N sz)%Z
+              then ret (IM.add k 0 mem, k)
+              else raiseOOM "Not enough memory."
+          | None => ret (IM.add k 0 mem, k)
+          end
+      end.
+
+  Variant AllocC : Type -> Type :=
+    | allocC (m : memory) : AllocC (unit + {k | IM.mem k m = false /\ ((exists sz, memory_size = Some sz /\ (k <= Z.of_N sz)%Z) \/ memory_size = None)}).
+
+  Definition do_alloc {E} `{OOME -< E} (mem : memory) : ctree E AllocC (memory * Z) :=
+    res <- branch (allocC mem);;
+    match res with
+    | inl x => raiseOOM "Not enough memory."
+    | inr x =>
+        let k := proj1_sig x in
+        ret (IM.add k 0 mem, k)
     end.
 
-Variant AllocC : Type -> Type :=
-  | allocC (m : memory) : AllocC (unit + {k | IM.mem k m = false /\ ((exists sz, memory_size = Some sz /\ (k <= sz)%Z) \/ memory_size = None)}).
+  Definition handle_mem_spec {E} `{OOME -< E} `{FailureE -< E} : MemE ~> Monads.stateT memory (ctree E AllocC) :=
+    fun _ e mem =>
+      match e with
+      | LoadE k =>
+          match IM.find k mem with
+          | Some v => ret (mem, v)
+          | None => raise "Load from unallocated address."
+          end
+      | StoreE k v =>
+          match IM.find k mem with
+          | Some _ =>
+              let mem' := IM.add k v mem in
+              ret (mem', tt)
+          | None => raise "Store to unallocated address."
+          end
+      | AllocE => do_alloc mem
+      end.
 
-Definition do_alloc {E} `{OOME -< E} (mem : memory) : ctree E AllocC (memory * Z) :=
-  res <- branch (allocC mem);;
-  match res with
-  | inl x => raiseOOM "Not enough memory."
-  | inr x =>
-      let k := proj1_sig x in
-      ret (IM.add k 0 mem, k)
-  end.
-
-Definition handle_mem_spec {E} `{OOME -< E} `{FailureE -< E} : MemE ~> Monads.stateT memory (ctree E AllocC) :=
-  fun _ e mem =>
-    match e with
-    | LoadE k =>
-        match IM.find k mem with
-        | Some v => ret (mem, v)
-        | None => raise "Load from unallocated address."
-        end
-    | StoreE k v =>
-        match IM.find k mem with
-        | Some _ =>
-            let mem' := IM.add k v mem in
-            ret (mem', tt)
-        | None => raise "Store to unallocated address."
-        end
-    | AllocE => do_alloc mem
-    end.
-
-Program Definition handle_AllocC {E} `{FailureE -< E} : AllocC ~> ctree E void1 :=
-  fun _ e => _.
-Next Obligation.
-  destruct e.
-  refine
-    (let k := next_key m in
-     match memory_size with
-     | Some sz => _
-     | None => _
-     end).
-  - (* Finite memory *)
-    destruct (Z_lt_le_dec sz k).
-    + (* Out of memory *)
-      apply (ret (inl tt)).
-    + refine (ret (inr _)).
+  Program Definition handle_AllocC {E} `{FailureE -< E} : AllocC ~> ctree E void1 :=
+    fun _ e => _.
+  Next Obligation.
+    destruct e.
+    refine
+      (let k := next_key m in
+       match memory_size with
+       | Some sz => _
+       | None => _
+       end).
+    - (* Finite memory *)
+      destruct (Z_lt_le_dec (Z.of_N sz) k).
+      + (* Out of memory *)
+        apply (ret (inl tt)).
+      + refine (ret (inr _)).
+        exists (next_key m).
+        destruct (IM.mem (elt:=nat) (next_key m) m) eqn:MEM.
+        * (* Contradiction *)
+          apply IM.mem_2 in MEM.
+          apply next_key_correct in MEM.
+          lia.
+        * split; auto.
+          left.
+          exists sz; split; auto; lia.
+    - (* Infinite memory *)
+      refine (ret (inr _)).
       exists (next_key m).
       destruct (IM.mem (elt:=nat) (next_key m) m) eqn:MEM.
       * (* Contradiction *)
@@ -380,52 +393,41 @@ Next Obligation.
         apply next_key_correct in MEM.
         lia.
       * split; auto.
-        left.
-        exists sz; split; auto; lia.
-  - (* Infinite memory *)
-    refine (ret (inr _)).
-    exists (next_key m).
-    destruct (IM.mem (elt:=nat) (next_key m) m) eqn:MEM.
-    * (* Contradiction *)
-      apply IM.mem_2 in MEM.
-      apply next_key_correct in MEM.
-      lia.
-    * split; auto.
-Defined.
+  Defined.
 
-Definition handle_mem_exec {E} `{FailureE -< E} `{OOME -< E} : MemE ~> Monads.stateT memory (ctree E void1) :=
-  fun _ e mem =>
-    Fold.refine handle_AllocC (@handle_mem_spec E _ _ _ e mem).
+  Definition handle_mem_exec {E} `{FailureE -< E} `{OOME -< E} : MemE ~> Monads.stateT memory (ctree E void1) :=
+    fun _ e mem =>
+      Fold.refine handle_AllocC (@handle_mem_spec E _ _ _ e mem).
 
-Notation Effin := (MemE +' FailureE +' OOME).
-Notation Bspec := AllocC.
-Notation Bexec := void1.
-Notation Effout := (FailureE +' OOME).
+  Notation Effin := (MemE +' FailureE +' OOME).
+  Notation Bspec := AllocC.
+  Notation Bexec := void1.
+  Notation Effout := (FailureE +' OOME).
 
-#[global] Instance Functor_VoidE : Functor void1.
-split.
-intros A B X H.
-destruct H.
-Defined.
+  #[global] Instance Functor_VoidE : Functor void1.
+  split.
+  intros A B X H.
+  destruct H.
+  Defined.
 
-#[global] Instance Functor_Bexec : Functor Bexec.
-try typeclasses eauto.
-Defined.
+  #[global] Instance Functor_Bexec : Functor Bexec.
+  try typeclasses eauto.
+  Defined.
 
-(* #[global] Instance Functor_AllocC : Functor AllocC. *)
-(* split. *)
-(* intros A B X H. *)
-(* inversion H; subst. *)
-(* forward X. *)
-(* exists (next_key m). *)
-(* destruct (IM.mem (elt:=nat) (next_key m) m) eqn:MEM; auto. *)
-(* apply IM.mem_2 in MEM. *)
-(* apply next_key_correct in MEM. *)
-(* lia. *)
+  (* #[global] Instance Functor_AllocC : Functor AllocC. *)
+  (* split. *)
+  (* intros A B X H. *)
+  (* inversion H; subst. *)
+  (* forward X. *)
+  (* exists (next_key m). *)
+  (* destruct (IM.mem (elt:=nat) (next_key m) m) eqn:MEM; auto. *)
+  (* apply IM.mem_2 in MEM. *)
+  (* apply next_key_correct in MEM. *)
+  (* lia. *)
 
-(* Abort. *)
+  (* Abort. *)
 
-(* 
+  (* 
 Definition in_rel : prerel Effin Effin.
   intros A B e1 e2.
   destruct e1, e2.
@@ -469,305 +471,325 @@ Definition in_post_rel : postrel Effin Effin.
   - apply True.
 Defined.
 
- *)
+   *)
 
-Require Import Vellvm.Utils.Tactics.
+  Require Import Vellvm.Utils.Tactics.
 
-Import SSimNotations.
+  Import SSimNotations.
 
-Lemma spec_refines_raise E `{FailureE -< E} F `{FailureE -< F} C D X Y L s :
-  @ssim
-    E F C D X Y L
-    (@raise E C _ _ s)
-    (@raise F D _ _ s).
-Proof.
-  unfold raise.
-  eapply ssim_clo_bind.
-  2: intros [].
-  apply ssim_vis.
-  intros [].
-  Unshelve.
-  apply eq.
-Qed.
+  Lemma spec_refines_raise E `{FailureE -< E} F `{FailureE -< F} C D X Y L s :
+    @ssim
+      E F C D X Y L
+      (@raise E C _ _ s)
+      (@raise F D _ _ s).
+  Proof.
+    unfold raise.
+    eapply ssim_clo_bind.
+    2: intros [].
+    apply ssim_vis.
+    intros [].
+    Unshelve.
+    apply eq.
+  Qed.
 
-Lemma ssim_raise_ret E `{FailureE -< E} F C D X Y L s y :
-  ~ @ssim
-    E F C D X Y L
-    (@raise E C _ _ s)
-    (ret y).
-Proof.
-  intros CONTRA.
-  unfold raise in *.
-  (* NEED vis / ret inv *)
-  unfold CTree.trigger in *.
-  cbn in *.
-  rewrite bind_vis in CONTRA.
-  step in CONTRA.
-  cbn in *.
-Admitted.
+  Lemma ssim_raise_ret E `{FailureE -< E} F C D X Y L s y :
+    ~ @ssim
+      E F C D X Y L
+      (@raise E C _ _ s)
+      (ret y).
+  Proof.
+    intros CONTRA.
+    unfold raise in *.
+    (* NEED vis / ret inv *)
+    unfold CTree.trigger in *.
+    cbn in *.
+    rewrite bind_vis in CONTRA.
+    step in CONTRA.
+    cbn in *.
+  Admitted.
 
-Lemma ssim_ret_raise E F `{FailureE -< F} C D X Y L s y :
-  ~ @ssim
-    E F C D X Y L
-    (ret y)
-    (@raise F D _ _ s).
-Proof.
-  intros CONTRA.
-  unfold raise in *.
-  (* NEED vis / ret inv *)
-  unfold CTree.trigger in *.
-  cbn in *.
-  rewrite bind_vis in CONTRA.
-  step in CONTRA.
-  cbn in *.
-  specialize (CONTRA (val y) Stuck).
-  forward CONTRA.
-  constructor.
-  destruct CONTRA as (?&?&?&?&?).
-  apply trans_vis_inv in H0.
-  destruct H0 as [[] _].
-Qed.
+  Lemma ssim_ret_raise E F `{FailureE -< F} C D X Y L s y :
+    ~ @ssim
+      E F C D X Y L
+      (ret y)
+      (@raise F D _ _ s).
+  Proof.
+    intros CONTRA.
+    unfold raise in *.
+    (* NEED vis / ret inv *)
+    unfold CTree.trigger in *.
+    cbn in *.
+    rewrite bind_vis in CONTRA.
+    step in CONTRA.
+    cbn in *.
+    specialize (CONTRA (val y) Stuck).
+    forward CONTRA.
+    constructor.
+    destruct CONTRA as (?&?&?&?&?).
+    apply trans_vis_inv in H0.
+    destruct H0 as [[] _].
+  Qed.
 
-Lemma handle_mem_correct {T} (e : MemE T) (m : memory):
-  @ssim Effin Effin _ _ _ _ eq (handle_mem T e m) (handle_mem_spec T e m).
-Proof.
-  destruct e.
-  - cbn.
-    break_match_goal.
-    + apply ssim_ret; auto.
-    + apply spec_refines_raise.
-  - cbn.
-    break_match_goal.
-    + apply ssim_ret; auto.
-    + apply spec_refines_raise.
-  - cbn.
+  Lemma handle_mem_correct {T} (e : MemE T) (m : memory):
+    @ssim Effin Effin _ _ _ _ eq (handle_mem T e m) (handle_mem_spec T e m).
+  Proof.
+    destruct e.
+    - cbn.
+      break_match_goal.
+      + apply ssim_ret; auto.
+      + apply spec_refines_raise.
+    - cbn.
+      break_match_goal.
+      + apply ssim_ret; auto.
+      + apply spec_refines_raise.
+    - cbn.
+      unfold do_alloc.
+      rewrite bind_branch.
+      eapply ssim_br_r.
+      Unshelve.
+      2: {
+        refine
+          (let k := next_key m in
+           match memory_size with
+           | Some sz => _
+           | None => inr _
+           end).
+
+        - destruct (Z_lt_le_dec (Z.of_N sz) k);
+            [apply (inl tt) | right].
+
+          exists k.
+          destruct (IM.mem (elt:=nat) (next_key m) m) eqn:MEM;
+            try solve
+              [ apply IM.mem_2 in MEM;
+                apply next_key_correct in MEM;
+                lia
+              ];
+            split; auto.
+          left; eexists; split; eauto; subst k; try lia.
+        - exists k.
+          destruct (IM.mem (elt:=nat) (next_key m) m) eqn:MEM;
+            try solve
+              [ apply IM.mem_2 in MEM;
+                apply next_key_correct in MEM;
+                lia
+              ];
+            split; auto.
+      }
+      cbn.
+      destruct memory_size as [sz | sz]; cbn.
+      { (* Finite *)
+        destruct (Z_lt_le_dec (Z.of_N sz) (next_key m)) as [SZ | SZ].
+        + assert ((next_key m <=? Z.of_N sz)%Z = false) by lia; rewrite H.
+          unfold raiseOOM.
+          apply ssim_clo_bind_eq; [| intros []].
+          unfold CTree.trigger.
+          apply ssim_vis.
+          intros [].
+        + assert ((next_key m <=? Z.of_N sz)%Z = true) by lia; rewrite H.
+          cbn.
+          apply ssim_ret.
+          reflexivity.
+      }
+
+      { (* Infinite *)
+        apply ssim_ret.
+        reflexivity.
+      }
+  Qed.
+
+  #[global] Instance handle_AllocC_pure :
+    forall E `{FailureE -< E}
+      (X : Type) (c : Bspec X), Pure.pure_finite (@handle_AllocC E _ X c).
+  Proof.
+    intros E H X c.
+    destruct c.
+    cbn.
+    break_match_goal; try break_match_goal;
+      apply Pure.pure_finite_ret.
+  Qed.
+
+  Lemma handle_mem_correct' {T} (e : MemE T) (m : memory):
+    @ssim Effin Effin _ _ _ _ eq (handle_mem_exec T e m) (handle_mem_spec T e m).
+  Proof.
+    unfold handle_mem_exec.
+    apply refine_ctree_ssim;
+      typeclasses eauto.
+  Qed.
+
+  Import FoldCTree.
+
+  Lemma refine_trigger :
+    forall E B1 B2 X (h : B1 ~> ctree E B2) (e: E X),
+      refine h (trigger e : ctree E B1 X) ~ (trigger e : ctree E B2 X).
+  Proof.
+    intros E B1 B2 X h e.
+    unfold trigger.
+    setoid_rewrite refine_vis.
+    setoid_rewrite sb_guard.
+    setoid_rewrite refine_ret.
+    rewrite bind_ret_r.
+    reflexivity.
+  Qed.
+
+  Lemma refine_raiseOOM :
+    forall E `{OOME -< E} B1 B2 X (h : B1 ~> ctree E B2) msg1 msg2,
+      refine h (raiseOOM msg1 : ctree E B1 X) ~ (raiseOOM msg2 : ctree E B2 X).
+  Proof.
+    intros E H B1 B2 X h msg1 msg2.
+    unfold raiseOOM.
+    rewrite refine_bind.
+    apply sbisim_clo_bind_eq; [|intros []].
+    apply refine_trigger.
+  Qed.
+
+  Lemma refine_raise :
+    forall E `{FailureE -< E} B1 B2 X (h : B1 ~> ctree E B2) msg1 msg2,
+      refine h (raise msg1 : ctree E B1 X) ~ (raise msg2 : ctree E B2 X).
+  Proof.
+    intros E H B1 B2 X h msg1 msg2.
+    unfold raise.
+    rewrite refine_bind.
+    apply sbisim_clo_bind_eq; [|intros []].
+    apply refine_trigger.
+  Qed.
+
+  Lemma handle_mem_exec_correct {T} (e : MemE T) (m : memory):
+    @sbisim Effin Effin _ _ _ _ eq (handle_mem_exec T e m) (handle_mem T e m).
+  Proof.
+    unfold handle_mem_exec.
+    unfold handle_mem.
+    destruct e; cbn.
+    - break_match_goal; cbn.
+      + rewrite refine_ret.
+        reflexivity.
+      + unfold raise, trigger.
+        rewrite refine_bind.
+        apply sbisim_clo_bind_eq; [|intros []].
+        rewrite refine_vis.
+        unfold trigger.
+        setoid_rewrite sb_guard.
+        setoid_rewrite refine_ret.
+        setoid_rewrite bind_ret_r.
+        reflexivity.
+    - break_match_goal; cbn.
+      + rewrite refine_ret.
+        reflexivity.
+      + unfold raise, trigger.
+        rewrite refine_bind.
+        apply sbisim_clo_bind_eq; [|intros []].
+        rewrite refine_vis.
+        unfold trigger.
+        setoid_rewrite sb_guard.
+        setoid_rewrite refine_ret.
+        setoid_rewrite bind_ret_r.
+        reflexivity.
+    - unfold do_alloc.
+      rewrite refine_bind.
+      setoid_rewrite refine_br.
+      rewrite bind_bind.
+      setoid_rewrite sb_guard.
+      setoid_rewrite refine_ret.
+      setoid_rewrite bind_ret_l.
+      cbn.
+      destruct memory_size as [sz | ].
+      break_match_goal.
+      + setoid_rewrite bind_ret_l.
+        assert ((next_key m <=? Z.of_N sz)%Z = false) by lia; rewrite H.
+        apply refine_raiseOOM.
+      + rewrite bind_ret_l; cbn.
+        rewrite refine_ret.
+        assert ((next_key m <=? Z.of_N sz)%Z = true) by lia; rewrite H.
+        reflexivity.
+      + rewrite bind_ret_l; cbn.
+        rewrite refine_ret.
+        reflexivity.
+  Qed.
+
+  Lemma alloca_empty :
+    forall k,
+      ((exists sz, memory_size = Some sz /\ (k <= Z.of_N sz)%Z) \/ memory_size = None) ->
+      @ssim Effin Effin void1 _ _ _ eq (ret (IM.add k 0 (IM.empty _), k))
+        (handle_mem_spec Z (AllocE) (IM.empty _)).
+  Proof.
+    intros k BOUNDS.
+    cbn.
     unfold do_alloc.
     rewrite bind_branch.
     eapply ssim_br_r.
     Unshelve.
     2: {
-      refine
-        (let k := next_key m in
-         match memory_size with
-         | Some sz => _
-         | None => inr _
-         end).
-
-      - destruct (Z_lt_le_dec sz k);
-          [apply (inl tt) | right].
-
-        exists k.
-        destruct (IM.mem (elt:=nat) (next_key m) m) eqn:MEM;
-          try solve
-              [ apply IM.mem_2 in MEM;
-                apply next_key_correct in MEM;
-                lia
-              ];
-          split; auto.
-        left; eexists; split; eauto; subst k; try lia.
-      - exists k.
-        destruct (IM.mem (elt:=nat) (next_key m) m) eqn:MEM;
-          try solve
-              [ apply IM.mem_2 in MEM;
-                apply next_key_correct in MEM;
-                lia
-              ];
-          split; auto.
+      right.
+      exists k.
+      destruct (IM.mem (elt:=nat) k _) eqn:MEM;
+        try solve
+          [ apply IM.mem_2 in MEM;
+            apply next_key_correct in MEM;
+            lia
+          ];
+        split; auto.
     }
+
     cbn.
-    destruct (Z_lt_le_dec 10 (next_key m)) as [SZ | SZ].
-    + assert ((next_key m <=? 10)%Z = false) by lia; rewrite H.
-      unfold raiseOOM.
-      apply ssim_clo_bind_eq; [| intros []].
-      unfold CTree.trigger.
-      apply ssim_vis.
-      intros [].
-    + assert ((next_key m <=? 10)%Z = true) by lia; rewrite H.
-      cbn.
-      apply ssim_ret.
-      reflexivity.
-Qed.
-
-#[global] Instance handle_AllocC_pure :
-  forall E `{FailureE -< E}
-    (X : Type) (c : Bspec X), Pure.pure_finite (@handle_AllocC E _ X c).
-Proof.
-  intros E H X c.
-  destruct c.
-  cbn.
-  break_match_goal;
-    apply Pure.pure_finite_ret.
-Qed.
-
-Lemma handle_mem_correct' {T} (e : MemE T) (m : memory):
-  @ssim Effin Effin _ _ _ _ eq (handle_mem_exec T e m) (handle_mem_spec T e m).
-Proof.
-  unfold handle_mem_exec.
-  apply refine_ctree_ssim;
-    typeclasses eauto.
-Qed.
-
-Import FoldCTree.
-
-Lemma refine_trigger :
-  forall E B1 B2 X (h : B1 ~> ctree E B2) (e: E X),
-    refine h (trigger e : ctree E B1 X) ~ (trigger e : ctree E B2 X).
-Proof.
-  intros E B1 B2 X h e.
-  unfold trigger.
-  setoid_rewrite refine_vis.
-  setoid_rewrite sb_guard.
-  setoid_rewrite refine_ret.
-  rewrite bind_ret_r.
-  reflexivity.
-Qed.
-
-Lemma refine_raiseOOM :
-  forall E `{OOME -< E} B1 B2 X (h : B1 ~> ctree E B2) msg1 msg2,
-    refine h (raiseOOM msg1 : ctree E B1 X) ~ (raiseOOM msg2 : ctree E B2 X).
-Proof.
-  intros E H B1 B2 X h msg1 msg2.
-  unfold raiseOOM.
-  rewrite refine_bind.
-  apply sbisim_clo_bind_eq; [|intros []].
-  apply refine_trigger.
-Qed.
-
-Lemma refine_raise :
-  forall E `{FailureE -< E} B1 B2 X (h : B1 ~> ctree E B2) msg1 msg2,
-    refine h (raise msg1 : ctree E B1 X) ~ (raise msg2 : ctree E B2 X).
-Proof.
-  intros E H B1 B2 X h msg1 msg2.
-  unfold raise.
-  rewrite refine_bind.
-  apply sbisim_clo_bind_eq; [|intros []].
-  apply refine_trigger.
-Qed.
-
-Lemma handle_mem_exec_correct {T} (e : MemE T) (m : memory):
-  @sbisim Effin Effin _ _ _ _ eq (handle_mem_exec T e m) (handle_mem T e m).
-Proof.
-  unfold handle_mem_exec.
-  unfold handle_mem.
-  destruct e; cbn.
-  - break_match_goal; cbn.
-    + rewrite refine_ret.
-      reflexivity.
-    + unfold raise, trigger.
-      rewrite refine_bind.
-      apply sbisim_clo_bind_eq; [|intros []].
-      rewrite refine_vis.
-      unfold trigger.
-      setoid_rewrite sb_guard.
-      setoid_rewrite refine_ret.
-      setoid_rewrite bind_ret_r.
-      reflexivity.
-  - break_match_goal; cbn.
-    + rewrite refine_ret.
-      reflexivity.
-    + unfold raise, trigger.
-      rewrite refine_bind.
-      apply sbisim_clo_bind_eq; [|intros []].
-      rewrite refine_vis.
-      unfold trigger.
-      setoid_rewrite sb_guard.
-      setoid_rewrite refine_ret.
-      setoid_rewrite bind_ret_r.
-      reflexivity.
-  - unfold do_alloc.
-    rewrite refine_bind.
-    setoid_rewrite refine_br.
-    rewrite bind_bind.
-    setoid_rewrite sb_guard.
-    setoid_rewrite refine_ret.
-    setoid_rewrite bind_ret_l.
-    cbn.
-    break_match_goal.
-    + setoid_rewrite bind_ret_l.
-      assert ((next_key m <=? 10)%Z = false) by lia; rewrite H.
-      apply refine_raiseOOM.
-    + rewrite bind_ret_l; cbn.
-      rewrite refine_ret.
-      assert ((next_key m <=? 10)%Z = true) by lia; rewrite H.
-      reflexivity.
-Qed.
-
-Lemma alloca_empty :
-  forall k,
-  @ssim Effin Effin void1 _ _ _ eq (ret (IM.add k 0 (IM.empty _), k))
-      (handle_mem_spec Z (AllocE) (IM.empty _)).
-Proof.
-  intros k.
-  cbn.
-  unfold do_alloc.
-  rewrite bind_branch.
-  eapply ssim_br_r.
-  Unshelve.
-  2: {
-    exists k.
-    destruct (IM.mem (elt:=nat) k (IM.empty nat)) eqn:MEM; auto.
-  }
-
-  cbn.
-  apply ssim_ret.
-  reflexivity.
-Qed.
-
-Lemma load_succeeds_spec :
-  forall m k v,
-    IM.find k m = Some v <->
-      @ssim Effin Effin void1 _ _ _ eq (ret (m, v))
-        (handle_mem_spec nat (LoadE k) m).
-Proof.
-  intros m k v.
-  split.
-  { intros LUP.
-    cbn; rewrite LUP.
     apply ssim_ret.
-    auto.
-  }
-  { intros REF.
-    cbn in REF.
-    destruct (IM.find k m) eqn:LUP.
-    - apply ssim_ret_inv in REF.
-      apply val_eq_inv in REF; inv REF; auto.
-    - apply ssim_ret_l_inv in REF.
-      destruct REF as (?&?&?&?); subst.
-      unfold raise in H.
-      apply trans_trigger_inv in H.
-      destruct H as [[] _].
-  }
-Qed.
+    destruct BOUNDS; reflexivity.
+  Qed.
 
-Lemma load_fails_spec :
-  forall T m k,
-    IM.find k m = None <->
-      @ssim Effin Effin void1 _ T _ eq
-        (raise "Load from unallocated address.")
-        (handle_mem_spec _ (LoadE k) m).
-Proof.
-  intros T m k.
-  split.
-  { intros LUP.
-    cbn; rewrite LUP.
-    apply spec_refines_raise.
-  }
-  { intros REF.
-    cbn in REF.
-    destruct (IM.find k m) eqn:LUP; auto.
-    apply ssim_raise_ret in REF.
-    contradiction.
-  }
-Qed.
+  Lemma load_succeeds_spec :
+    forall m k v,
+      IM.find k m = Some v <->
+        @ssim Effin Effin void1 _ _ _ eq (ret (m, v))
+          (handle_mem_spec nat (LoadE k) m).
+  Proof.
+    intros m k v.
+    split.
+    { intros LUP.
+      cbn; rewrite LUP.
+      apply ssim_ret.
+      auto.
+    }
+    { intros REF.
+      cbn in REF.
+      destruct (IM.find k m) eqn:LUP.
+      - apply ssim_ret_inv in REF.
+        apply val_eq_inv in REF; inv REF; auto.
+      - apply ssim_ret_l_inv in REF.
+        destruct REF as (?&?&?&?); subst.
+        unfold raise in H.
+        apply trans_trigger_inv in H.
+        destruct H as [[] _].
+    }
+  Qed.
 
-Lemma store_succeeds_spec :
-  forall m m' k v,
-    IM.mem k m = true /\
-      m' = IM.add k v m
-    <->
-      @ssim Effin Effin void1 _ _ _ eq
-        (ret (m', tt))
-        (handle_mem_spec _ (StoreE k v) m).
+  Lemma load_fails_spec :
+    forall T m k,
+      IM.find k m = None <->
+        @ssim Effin Effin void1 _ T _ eq
+          (raise "Load from unallocated address.")
+          (handle_mem_spec _ (LoadE k) m).
+  Proof.
+    intros T m k.
+    split.
+    { intros LUP.
+      cbn; rewrite LUP.
+      apply spec_refines_raise.
+    }
+    { intros REF.
+      cbn in REF.
+      destruct (IM.find k m) eqn:LUP; auto.
+      apply ssim_raise_ret in REF.
+      contradiction.
+    }
+  Qed.
+
+  Lemma store_succeeds_spec :
+    forall m m' k v,
+      IM.mem k m = true /\
+        m' = IM.add k v m
+      <->
+        @ssim Effin Effin void1 _ _ _ eq
+          (ret (m', tt))
+          (handle_mem_spec _ (StoreE k v) m).
 
   (*
 
@@ -779,699 +801,839 @@ Lemma store_succeeds_spec :
            r1 = r2 /\
              fst r2 = m'
         ) *)
-Proof.
-  intros m m' k v.
-  split.
-  { intros [MEM ADD]; subst.
-    cbn.
-    apply IM.mem_2 in MEM.
-    destruct MEM.
-    erewrite IM.find_1; eauto.
-    apply ssim_ret.
-    auto.
-  }
-  { intros REF.
-    cbn in REF.
-    destruct (IM.find k m) eqn:LUP; subst.
-    - apply ssim_ret_inv in REF.
-      apply val_eq_inv in REF.
-      inv REF.
-      split; auto.
-      apply IM.mem_1.
-      exists n.
-      eapply IM.find_2; eauto.
-    - apply ssim_ret_raise in REF; contradiction.
-  }
-Qed.
+  Proof.
+    intros m m' k v.
+    split.
+    { intros [MEM ADD]; subst.
+      cbn.
+      apply IM.mem_2 in MEM.
+      destruct MEM.
+      erewrite IM.find_1; eauto.
+      apply ssim_ret.
+      auto.
+    }
+    { intros REF.
+      cbn in REF.
+      destruct (IM.find k m) eqn:LUP; subst.
+      - apply ssim_ret_inv in REF.
+        apply val_eq_inv in REF.
+        inv REF.
+        split; auto.
+        apply IM.mem_1.
+        exists n.
+        eapply IM.find_2; eauto.
+      - apply ssim_ret_raise in REF; contradiction.
+    }
+  Qed.
 
-Lemma store_fails_spec :
-  forall T m k v,
-    IM.find k m = None
-    <->
-      @ssim Effin Effin void1 _ T _ eq
-        (raise "Store to unallocated address.")
-        (handle_mem_spec _ (StoreE k v) m).
-Proof.
-  intros T m k v.
-  split.
-  { intros LUP.
-    cbn; rewrite LUP.
-    apply spec_refines_raise.
-  }
-  { intros REF.
-    cbn in REF.
-    destruct (IM.find k m) eqn:LUP; auto.
-    apply ssim_raise_ret in REF.
-    contradiction.
-  }
-Qed.
+  Lemma store_fails_spec :
+    forall T m k v,
+      IM.find k m = None
+      <->
+        @ssim Effin Effin void1 _ T _ eq
+          (raise "Store to unallocated address.")
+          (handle_mem_spec _ (StoreE k v) m).
+  Proof.
+    intros T m k v.
+    split.
+    { intros LUP.
+      cbn; rewrite LUP.
+      apply spec_refines_raise.
+    }
+    { intros REF.
+      cbn in REF.
+      destruct (IM.find k m) eqn:LUP; auto.
+      apply ssim_raise_ret in REF.
+      contradiction.
+    }
+  Qed.
 
-Lemma alloc_spec :
-  forall (m m' : memory) k,
-    IM.mem k m = false /\
-      m' = IM.add k 0 m
-    <->
-      @ssim Effin Effin void1 _ _ _ eq
-        (ret (m', k))
-        (handle_mem_spec Z (AllocE) m).
-(* (fun r1 r2 =>
+  Lemma alloc_spec :
+    forall (m m' : memory) k,
+      IM.mem k m = false /\
+        m' = IM.add k 0 m /\
+        ((exists sz, memory_size = Some sz /\ (k <= Z.of_N sz)%Z) \/ memory_size = None)
+      <->
+        @ssim Effin Effin void1 _ _ _ eq
+          (ret (m', k))
+          (handle_mem_spec Z (AllocE) m).
+  (* (fun r1 r2 =>
         r1 = r2 /\
           let m2 := fst r2 in
           let k2 := snd r2 in
           k2 = k /\
             m2 = add k 0 m) *)
-Proof.
-  intros m m' k.
-  split.
-  { intros [NMEM ADD].
-    cbn; unfold do_alloc.
-    rewrite bind_branch.
-    eapply ssim_br_r.
-    Unshelve.
-    2: {
-      exists k.
-      destruct (IM.mem (elt:=nat) k (IM.empty nat)) eqn:MEM; auto.
+  Proof.
+    intros m m' k.
+    split.
+    { intros [NMEM [ADD IN]].
+      cbn; unfold do_alloc.
+      rewrite bind_branch.
+      eapply ssim_br_r.
+      Unshelve.
+      2: {
+        right.
+        exists k.
+        destruct (IM.mem (elt:=nat) k (IM.empty nat)) eqn:MEM; auto.
+      }
+
+      cbn; subst.
+      apply ssim_ret.
+      reflexivity.
     }
+    { intros REF.
+      cbn in *.
+      unfold do_alloc in *.
+      apply ssim_ret_l_inv in REF.
+      destruct REF as (?&?&?&?); subst.
+      rewrite bind_branch in H.
+      apply trans_br_inv in H.
+      destruct H as (?&?).
+      break_match_hyp.
+      inv H. (* Contradition *)
+      apply trans_ret_inv in H.
+      destruct H.
+      apply val_eq_inv in H0. inv H0.
+      destruct s; subst; cbn in *.
+      tauto.
+    }
+  Qed.
 
-    cbn; subst.
-    apply ssim_ret.
-    reflexivity.
-  }
-  { intros REF.
-    cbn in *.
-    unfold do_alloc in *.
-    apply ssim_ret_l_inv in REF.
-    destruct REF as (?&?&?&?); subst.
-    rewrite bind_branch in H.
-    apply trans_br_inv in H.
-    destruct H as (?&?).
-    apply trans_ret_inv in H.
-    destruct H.
-    apply val_eq_inv in H0. inv H0.
-    destruct x; subst; cbn in *.
-    eauto.
-  }
-Qed.
-
-Lemma alloc_spec_exists :
-  forall (m : memory),
-  exists m' k,
-    IM.mem k m = false /\
-      m' = IM.add k 0 m /\
-      @ssim Effin Effin void1 _ _ _ eq
-        (ret (m', k))
-        (handle_mem_spec Z (AllocE) m).
-(* (fun r1 r2 =>
+  (* Not true in a finite setting *)
+  Lemma alloc_spec_exists :
+    forall (m : memory),
+      memory_size = None ->
+      exists m' k,
+        IM.mem k m = false /\
+          m' = IM.add k 0 m /\
+          @ssim Effin Effin void1 _ _ _ eq
+            (ret (m', k))
+            (handle_mem_spec Z (AllocE) m).
+  (* (fun r1 r2 =>
          r1 = r2 /\
            fst r2 = m' /\
            snd r2 = k) *)
-Proof.
-  intros m.
-  destruct (IM.mem (next_key m) m) eqn:MEM; auto.
-  apply IM.mem_2 in MEM.
-  apply next_key_correct in MEM.
-  lia.
+  Proof.
+    intros m.
+    destruct (IM.mem (next_key m) m) eqn:MEM; auto.
+    apply IM.mem_2 in MEM.
+    apply next_key_correct in MEM.
+    lia.
 
-  exists (IM.add (next_key m) 0 m), (next_key m).
-  split; auto.
-  split; auto.
+    exists (IM.add (next_key m) 0 m), (next_key m).
+    split; auto.
+    split; auto.
 
-  cbn.
-  unfold do_alloc.
-  rewrite bind_branch.
-  
-  cbn.
-  eapply ssim_br_r.
-  Unshelve.
-  2: {
-    exists (next_key m); auto.
-  }
-
-  cbn.
-  apply ssim_ret.
-  reflexivity.
-Qed.
-
-Definition double_alloc : ctree MemE void1 bool
-  := k <- trigger AllocE;;
-     p <- trigger AllocE;;
-     ret (Z.eqb k p).
-
-
-Lemma next_key_not_member :
-  forall {A} (m : IM.t A),
-    IM.mem (next_key m) m = false.
-Proof.
-  intros A m.
-  destruct (IM.mem (next_key m) m) eqn:MEM; auto.
-  apply IM.mem_2 in MEM.
-  apply next_key_correct in MEM.
-  lia.
-Qed.
-
-Lemma alloc_sigma :
-  forall {A} (m : IM.t A),
-    {k | IM.mem k m = false}.
-Proof.
-  intros A m.
-  exists (next_key m).
-  eapply next_key_not_member.
-Defined.
-
-
-(* Definition interp_state {E B M S} *)
-(*            {FM : Functor M} {MM : Monad M} *)
-(*            {IM : MonadIter M} *)
-(*            (h : E ~> Monads.stateT S M) : *)
-(*   ctree E B ~> Monads.stateT S M := interp h. *)
-
-Import Monads.
-
-#[global] Instance ctree_monad {E B} : Monad (ctree E B).
-split.
-- intros.
-  apply ret; apply X.
-- intros t u X X0.
-  eapply bind.
-  apply X.
-  apply X0.
-Defined.
-
-#[global] Instance MonadStepState {S M} `{HM : Monad M} `{MS : MonadStep M} : MonadStep (Monads.stateT S M).
-red.
-intros s.
-eapply bind.
-apply mstep.
-intros _.
-apply (ret (s, tt)).
-Defined.
-
-#[global] Instance MonadStuckState {S M} `{HM : Monad M} `{MS : MonadStuck M} : MonadStuck (Monads.stateT S M).
-red.
-intros X.
-red.
-intros s.
-apply mstuck.
-Defined.
-
-#[global] Instance MonadBrState {B S M} `{HM : Monad M} `{MB : MonadBr B M} : MonadBr B (stateT S M).
-red.
-intros X b s.
-apply mbr in b.
-eapply fmap; cycle 1; eauto.
-Defined.
-
-Lemma alloc_disjoint :
-  exists m,
-    @ssim Effin Effin void1 Bspec (memory * bool)%type (memory * bool)%type eq
-      (ret (m, false))
-      (interp_state handle_mem_spec double_alloc (IM.empty _)).
-Proof.
-  eexists.
-  unfold double_alloc.
-  repeat setoid_rewrite interp_state_bind.
-  setoid_rewrite interp_state_trigger.
-  repeat setoid_rewrite bind_bind.
-  rewrite bind_branch.
-  apply ssim_br_r with (x:=alloc_sigma _); cbn.
-  rewrite bind_ret_l.
-  rewrite bind_guard.
-  apply ssim_guard_r.
-  rewrite bind_ret_l.
-  rewrite bind_branch.
-  apply ssim_br_r with (x:=alloc_sigma _); cbn.
-  rewrite bind_ret_l.
-  rewrite bind_guard.
-  apply ssim_guard_r.
-  rewrite bind_ret_l.
-  rewrite interp_state_ret; cbn.
-  apply ssim_ret.
-  reflexivity.
-Qed.
-
-Lemma mem_add_eq {a}: forall k v (m: IM.t a),
-    IM.mem k (IM.add k v m) = true.
-Proof using.
-  intros.
-  cbn.
-  apply IM.Raw.Proofs.mem_1.
-  apply IM.Raw.Proofs.add_bst, IM.is_bst.
-  rewrite IM.Raw.Proofs.add_in; auto.
-Qed.
-
-Lemma find_add_eq {a}: forall k v (m: IM.t a),
-    IM.find k (IM.add k v m) = Some v.
-Proof using.
-  intros.
-  apply IM.find_1.
-  apply IM.add_1; auto.
-Qed.
-
-Lemma mem_add_neq {a}: forall k1 k2 v (m: IM.t a),
-    k1 <> k2 ->
-    IM.mem k1 (IM.add k2 v m) = IM.mem k1 m.
-Proof using.
-  intros.
-  cbn.
-Admitted.
-
-Lemma alloc_disjoint' :
-  forall m,
-    @ssim Effin Effin Bspec Bexec bool bool eq
-      (fmap snd (interp_state handle_mem_spec double_alloc m))
-      (ret false).
-Proof.
-  intros m.
-  Opaque IM.mem.
-  setoid_rewrite interp_state_bind.
-  setoid_rewrite interp_state_bind.
-  setoid_rewrite interp_state_trigger.
-  repeat setoid_rewrite map_bind.
-  cbn.
-  repeat setoid_rewrite bind_bind; cbn.
-  rewrite bind_branch.
-  apply ssim_br_l.
-  intros [k KSPEC].
-
-  rewrite bind_ret_l; cbn.
-  rewrite bind_guard.
-  apply ssim_guard_l.
-  rewrite bind_ret_l; cbn.
-
-  rewrite bind_branch.
-  apply ssim_br_l.
-  intros [p PSPEC].
-
-  rewrite bind_ret_l; cbn.
-  rewrite bind_guard.
-  apply ssim_guard_l.
-  rewrite bind_ret_l; cbn.
-
-  rewrite interp_state_ret.
-  rewrite map_ret.
-  cbn.
-
-  destruct (Z.eq_dec k p) as [EQ | NEQ]; cbn in *; subst.
-  rewrite mem_add_eq in PSPEC; try discriminate.
-
-  assert ((k =? p)%Z = false) by lia.
-  rewrite H.
-  apply ssim_ret.
-  reflexivity.
-Qed.
-
-
-Lemma double_alloc_spec :
-  forall m m' b,
-    (b = false /\
-       exists k1 k2,
-         m' = IM.add k2 0 (IM.add k1 0 m) /\
-           k1 <> k2 /\
-           IM.mem k1 m = false /\
-           IM.mem k2 m = false) ->
-    @ssim Effin Effin void1 Bspec (memory * bool)%type (memory * bool)%type eq
-      (ret (m', b))
-      (interp_state handle_mem_spec double_alloc m).
-Proof.
-  intros m m' b.
-  { intros [B K].
-    destruct K as (k1&k2&M'&NK1K2&MEM1&MEM2).
     cbn.
-    repeat setoid_rewrite interp_state_bind.
-    repeat setoid_rewrite interp_state_trigger.
-    repeat setoid_rewrite bind_bind.
-
+    unfold do_alloc.
     rewrite bind_branch.
-    apply ssim_br_r with (x:=exist _ k1 MEM1); cbn.
+    
+    cbn.
+    eapply ssim_br_r.
+    Unshelve.
+    2: {
+      right.
+      exists (next_key m); auto.
+    }
+
+    cbn.
+    apply ssim_ret.
+    reflexivity.
+  Qed.
+
+  Definition double_alloc : ctree MemE void1 bool
+    := k <- trigger AllocE;;
+       p <- trigger AllocE;;
+       ret (Z.eqb k p).
+
+
+  Lemma next_key_not_member :
+    forall {A} (m : IM.t A),
+      IM.mem (next_key m) m = false.
+  Proof.
+    intros A m.
+    destruct (IM.mem (next_key m) m) eqn:MEM; auto.
+    apply IM.mem_2 in MEM.
+    apply next_key_correct in MEM.
+    lia.
+  Qed.
+
+  Definition memory_size_ge (sz : Z) : bool :=
+    match memory_size with
+    | Some x => (sz <=? Z.of_N x)%Z
+    | None => true
+    end.
+
+  (* None means infinite memory is available *)
+  Definition free_memory_amount (m : memory) : option N :=
+    match memory_size with
+    | None => None
+    | Some sz =>
+        Some (sz - N.of_nat (IM.cardinal m))%N
+    end.
+
+  Definition bytes_available (m : memory) (n : N) : bool :=
+    match free_memory_amount m with
+    | None => true
+    | Some sz =>
+        N.leb n sz
+    end.
+
+  Definition well_formed_memory (m : memory) : bool :=
+    match memory_size with
+    | None => true
+    | Some sz =>
+        match IM_greatest_key m with
+        | None => true
+        | Some k =>
+            (k <=? Z.of_N sz)%Z
+        end
+    end.
+
+  Lemma alloc_sigma :
+    forall (m : memory),
+      well_formed_memory m = true ->
+      bytes_available m 1%N = true ->
+      {k | IM.mem k m = false /\ ((exists sz, memory_size = Some sz /\ (k <= Z.of_N sz)%Z) \/ memory_size = None)}.
+  Proof.
+    intros m WF AVAIL.
+    unfold bytes_available, free_memory_amount in *.
+    unfold well_formed_memory in WF.
+    destruct memory_size as [sz|].
+    { (* Finite *)
+      (* WF and AVAIL should mean that there is a free slot in memory *)
+      destruct (IM_greatest_key m) eqn:GREAT.
+      - (* There's an unfilled slot in memory... *)
+        admit.
+      - pose proof GREAT as Heqo.
+        apply IM_greatest_key_none in Heqo.
+        exists (next_key m). repeat split; auto.
+        apply F.not_mem_in_iff.
+        intros IN.
+        destruct IN.
+        apply Heqo in H; auto.
+        left.
+        exists sz; eauto.
+        repeat red in IN.
+        split; auto.
+
+        apply cardinal_Empty in Heqo.
+        rewrite Heqo in AVAIL.
+        unfold next_key.
+        rewrite GREAT.
+        lia.
+    }
+
+    (* Infinite *)
+    exists (next_key m).
+    split; auto.
+    eapply next_key_not_member.
+  Admitted.
+
+
+  (* Definition interp_state {E B M S} *)
+  (*            {FM : Functor M} {MM : Monad M} *)
+  (*            {IM : MonadIter M} *)
+  (*            (h : E ~> Monads.stateT S M) : *)
+  (*   ctree E B ~> Monads.stateT S M := interp h. *)
+
+  Import Monads.
+
+  #[global] Instance ctree_monad {E B} : Monad (ctree E B).
+  split.
+  - intros.
+    apply ret; apply X.
+  - intros t u X X0.
+    eapply bind.
+    apply X.
+    apply X0.
+  Defined.
+
+  #[global] Instance MonadStepState {S M} `{HM : Monad M} `{MS : MonadStep M} : MonadStep (Monads.stateT S M).
+  red.
+  intros s.
+  eapply bind.
+  apply mstep.
+  intros _.
+  apply (ret (s, tt)).
+  Defined.
+
+  #[global] Instance MonadStuckState {S M} `{HM : Monad M} `{MS : MonadStuck M} : MonadStuck (Monads.stateT S M).
+  red.
+  intros X.
+  red.
+  intros s.
+  apply mstuck.
+  Defined.
+
+  #[global] Instance MonadBrState {B S M} `{HM : Monad M} `{MB : MonadBr B M} : MonadBr B (stateT S M).
+  red.
+  intros X b s.
+  apply mbr in b.
+  eapply fmap; cycle 1; eauto.
+  Defined.
+
+  Lemma alloc_disjoint :
+    (* There's enough memory for both allocations *)
+    memory_size_ge 2 = true ->
+    exists m,
+      @ssim Effin Effin void1 Bspec (memory * bool)%type (memory * bool)%type eq
+        (ret (m, false))
+        (interp_state handle_mem_spec double_alloc (IM.empty _)).
+  Proof.
+    intros FITS.
+    unfold memory_size_ge in FITS.
+
+    (* First allocation *)
+    pose proof alloc_sigma (IM.empty nat) as ALLOC1.
+
+    forward ALLOC1.
+    { unfold well_formed_memory.
+      break_match_goal; auto.
+    }
+
+    forward ALLOC1.
+    { unfold bytes_available, free_memory_amount, memory_size_ge.
+      break_inner_match_goal; auto.
+      pose proof (@cardinal_Empty _ (IM.empty nat)).
+      destruct H.
+      rewrite H; eauto.
+      cbn in *.
+      apply N.leb_le.
+      lia.
+    }
+
+    (* Second allocation *)
+    pose proof alloc_sigma (IM.add (proj1_sig ALLOC1) 0 (IM.empty nat)) as ALLOC2.
+
+    forward ALLOC2.
+    { unfold well_formed_memory.
+      break_match_goal; cbn; auto.
+      destruct ALLOC1 as (?&?&[?|?]); [|discriminate]; cbn in *.
+      destruct e0 as (?&?&?).
+      inv H.
+      lia.
+    }
+
+    forward ALLOC2.
+    { unfold bytes_available, free_memory_amount.
+      break_inner_match_goal; cbn; auto.
+      apply N.leb_le.
+      lia.
+    }
+
+    exists (IM.add (proj1_sig ALLOC2) 0 (IM.add (proj1_sig ALLOC1) 0 (IM.empty nat))).
+
+    unfold double_alloc.
+    repeat setoid_rewrite interp_state_bind.
+    setoid_rewrite interp_state_trigger.
+    repeat setoid_rewrite bind_bind.
+    rewrite bind_branch.
+
+    cbn.
+    apply ssim_br_r with (x:=inr ALLOC1); cbn.
     rewrite bind_ret_l.
-    rewrite bind_guard.
-    eapply ssim_guard_r.
-    repeat setoid_rewrite bind_ret_l.
-
-    rewrite bind_branch; cbn.
-    assert (IM.mem (elt:=nat) k2 (IM.add k1 0 m) = false) as MEM2'.
-    rewrite mem_add_neq; eauto.
-
-    apply ssim_br_r with (x:=exist _ k2 MEM2'); cbn.
     rewrite bind_guard.
     apply ssim_guard_r.
     rewrite bind_ret_l.
-    rewrite interp_state_ret.
-    cbn.
-    subst.
+    rewrite bind_branch.
+
+    apply ssim_br_r with (x:=inr ALLOC2); cbn.
+    rewrite bind_ret_l.
+    rewrite bind_guard.
+    apply ssim_guard_r.
+    rewrite bind_ret_l.
+    rewrite interp_state_ret; cbn.
     apply ssim_ret.
-
-    assert ((k1 =? k2)%Z = false) by lia.
-    rewrite H.
+    assert (proj1_sig ALLOC1 <> proj1_sig ALLOC2).
+    { destruct ALLOC1 as (?&?&?).
+      destruct ALLOC2 as (?&?&?).
+      cbn in *.
+      intros CONTRA.
+      subst.
+      pose proof IM.Raw.Proofs.MX.elim_compare_eq (@eq_refl _ x0).
+      destruct H.
+      rewrite H in e0.
+      discriminate.
+    }
+    assert (proj1_sig ALLOC1 =? proj1_sig ALLOC2 = false)%Z by lia.
+    setoid_rewrite H0.
     reflexivity.
-  }
-Qed.
+  Qed.
 
-Definition store_prog (v : nat) : ctree MemE Bspec nat :=
-  k <- trigger AllocE;;
-  trigger (StoreE k v);;
-  trigger (LoadE k).
+  Lemma mem_add_eq {a}: forall k v (m: IM.t a),
+      IM.mem k (IM.add k v m) = true.
+  Proof using.
+    intros.
+    cbn.
+    apply IM.Raw.Proofs.mem_1.
+    apply IM.Raw.Proofs.add_bst, IM.is_bst.
+    rewrite IM.Raw.Proofs.add_in; auto.
+  Qed.
 
-Lemma alloc_lemma :
-  forall m m_final k,
-    IM.mem k m = false ->
-    m_final = IM.add k 0 m ->
-    @ssim Effin Effin Bspec Bspec (memory * IM.key)%type (memory * IM.key)%type eq
-      (ret (m_final, k))
-      (interp_state handle_mem_spec (trigger AllocE : ctree MemE Bspec Z) m).
-Proof.
-  intros m m_final k MEM FINAL.
-  setoid_rewrite interp_state_trigger.
-  cbn.
+  Lemma find_add_eq {a}: forall k v (m: IM.t a),
+      IM.find k (IM.add k v m) = Some v.
+  Proof using.
+    intros.
+    apply IM.find_1.
+    apply IM.add_1; auto.
+  Qed.
 
-  unfold do_alloc.
-  rewrite bind_branch.
-  rewrite bind_br.
-  eapply ssim_br_r with (x:=exist _ k MEM); cbn.
-  rewrite bind_ret_l.
-  apply ssim_guard_r.
-  apply ssim_ret.
-  subst.
-  reflexivity.
-Qed.
+  Lemma mem_add_neq {a}: forall k1 k2 v (m: IM.t a),
+      k1 <> k2 ->
+      IM.mem k1 (IM.add k2 v m) = IM.mem k1 m.
+  Proof using.
+    intros.
+    cbn.
+  Admitted.
 
-Lemma alloc_lemma' :
-  forall m,
-    @ssim Effin Effin Bspec Bspec (memory * IM.key)%type (memory * IM.key)%type eq
-      (ret (IM.add (next_key m) 0 m, next_key m))
-      (interp_state handle_mem_spec (trigger AllocE : ctree MemE Bspec Z) m).
-Proof.
-  intros m.
-  eapply alloc_lemma.
-  apply next_key_not_member.
-  reflexivity.
-Qed.
+  Lemma alloc_disjoint' :
+    forall m,
+      @ssim Effin Effin Bspec Bexec bool bool eq
+        (fmap snd (interp_state handle_mem_spec double_alloc m))
+        (ret false).
+  Proof.
+    intros m.
+    Opaque IM.mem.
+    setoid_rewrite interp_state_bind.
+    setoid_rewrite interp_state_bind.
+    setoid_rewrite interp_state_trigger.
+    repeat setoid_rewrite map_bind.
+    cbn.
+    repeat setoid_rewrite bind_bind; cbn.
+    rewrite bind_branch.
+    apply ssim_br_l.
+    intros [_ | [k KSPEC]].
+    { (* TODO: OOM case. Adjust this when we can define an OOM
+         refinement relation. *)
+      admit.
+    }
 
-Lemma store_succ_lemma :
-  forall m m_final k v,
-    IM.mem k m = true ->
-    m_final = IM.add k v m ->
-    (interp_state (@handle_mem_spec Effin _) (trigger (StoreE k v) : ctree MemE Bspec unit) m) ~
-      (ret (m_final, tt) : ctree Effin Bspec (memory * unit)%type).
-Proof.
-  intros m m_final k v MEM FINAL.
-  setoid_rewrite interp_state_trigger.
-  cbn.
-  apply IM.mem_2 in MEM.
-  destruct MEM.
-  erewrite IM.find_1; eauto.
-  rewrite bind_ret_l.
+    rewrite bind_ret_l; cbn.
+    rewrite bind_guard.
+    apply ssim_guard_l.
+    rewrite bind_ret_l; cbn.
 
-  apply sb_guard_l.
-  subst.
-  reflexivity.
-Qed.
+    rewrite bind_branch.
+    apply ssim_br_l.
+    intros [_ | [p [PSPEC PSPEC']]].
+    { (* TODO: OOM case. Adjust this when we can define an OOM
+         refinement relation. *)
+      admit.
+    }
 
-Lemma load_succ_lemma :
-  forall m k v,
-    IM.find k m = Some v ->
-    (interp_state (@handle_mem_spec Effin _) (trigger (LoadE k) : ctree MemE Bspec nat) m) ~
-      (ret (m, v) : ctree Effin Bspec (memory * nat)%type).
-Proof.
-  intros m k v LUP.
-  setoid_rewrite interp_state_trigger.
-  cbn.
-  rewrite LUP.
-  rewrite bind_ret_l.
-  apply sb_guard_l.
-  reflexivity.
-Qed.
+    rewrite bind_ret_l; cbn.
+    rewrite bind_guard.
+    apply ssim_guard_l.
+    rewrite bind_ret_l; cbn.
 
-Ltac inj_pair2_existT :=
-  repeat
+    rewrite interp_state_ret.
+    rewrite map_ret.
+    cbn.
+
+    destruct (Z.eq_dec k p) as [EQ | NEQ]; cbn in *; subst.
+    rewrite mem_add_eq in PSPEC; try discriminate.
+
+    assert ((k =? p)%Z = false) by lia.
+    rewrite H.
+    apply ssim_ret.
+    reflexivity.
+  Admitted.
+
+
+  Lemma double_alloc_spec :
+    forall m m' b,
+      (b = false /\
+         bytes_available m 2%N = true /\
+         exists k1 k2,
+           m' = IM.add k2 0 (IM.add k1 0 m) /\
+             k1 <> k2 /\
+             IM.mem k1 m = false /\
+             IM.mem k2 m = false) ->
+      @ssim Effin Effin void1 Bspec (memory * bool)%type (memory * bool)%type eq
+        (ret (m', b))
+        (interp_state handle_mem_spec double_alloc m).
+  Proof.
+    intros m m' b.
+    { intros [B [AVAIL K]].
+      destruct K as (k1&k2&M'&NK1K2&MEM1&MEM2).
+      cbn.
+      repeat setoid_rewrite interp_state_bind.
+      repeat setoid_rewrite interp_state_trigger.
+      repeat setoid_rewrite bind_bind.
+
+      rewrite bind_branch.
+      apply ssim_br_r with (x:=exist _ k1 MEM1); cbn.
+      rewrite bind_ret_l.
+      rewrite bind_guard.
+      eapply ssim_guard_r.
+      repeat setoid_rewrite bind_ret_l.
+
+      rewrite bind_branch; cbn.
+      assert (IM.mem (elt:=nat) k2 (IM.add k1 0 m) = false) as MEM2'.
+      rewrite mem_add_neq; eauto.
+
+      apply ssim_br_r with (x:=exist _ k2 MEM2'); cbn.
+      rewrite bind_guard.
+      apply ssim_guard_r.
+      rewrite bind_ret_l.
+      rewrite interp_state_ret.
+      cbn.
+      subst.
+      apply ssim_ret.
+
+      assert ((k1 =? k2)%Z = false) by lia.
+      rewrite H.
+      reflexivity.
+    }
+  Qed.
+
+  Definition store_prog (v : nat) : ctree MemE Bspec nat :=
+    k <- trigger AllocE;;
+    trigger (StoreE k v);;
+    trigger (LoadE k).
+
+  Lemma alloc_lemma :
+    forall m m_final k,
+      IM.mem k m = false ->
+      m_final = IM.add k 0 m ->
+      @ssim Effin Effin Bspec Bspec (memory * IM.key)%type (memory * IM.key)%type eq
+        (ret (m_final, k))
+        (interp_state handle_mem_spec (trigger AllocE : ctree MemE Bspec Z) m).
+  Proof.
+    intros m m_final k MEM FINAL.
+    setoid_rewrite interp_state_trigger.
+    cbn.
+
+    unfold do_alloc.
+    rewrite bind_branch.
+    rewrite bind_br.
+    eapply ssim_br_r with (x:=exist _ k MEM); cbn.
+    rewrite bind_ret_l.
+    apply ssim_guard_r.
+    apply ssim_ret.
+    subst.
+    reflexivity.
+  Qed.
+
+  Lemma alloc_lemma' :
+    forall m,
+      @ssim Effin Effin Bspec Bspec (memory * IM.key)%type (memory * IM.key)%type eq
+        (ret (IM.add (next_key m) 0 m, next_key m))
+        (interp_state handle_mem_spec (trigger AllocE : ctree MemE Bspec Z) m).
+  Proof.
+    intros m.
+    eapply alloc_lemma.
+    apply next_key_not_member.
+    reflexivity.
+  Qed.
+
+  Lemma store_succ_lemma :
+    forall m m_final k v,
+      IM.mem k m = true ->
+      m_final = IM.add k v m ->
+      (interp_state (@handle_mem_spec Effin _) (trigger (StoreE k v) : ctree MemE Bspec unit) m) ~
+        (ret (m_final, tt) : ctree Effin Bspec (memory * unit)%type).
+  Proof.
+    intros m m_final k v MEM FINAL.
+    setoid_rewrite interp_state_trigger.
+    cbn.
+    apply IM.mem_2 in MEM.
+    destruct MEM.
+    erewrite IM.find_1; eauto.
+    rewrite bind_ret_l.
+
+    apply sb_guard_l.
+    subst.
+    reflexivity.
+  Qed.
+
+  Lemma load_succ_lemma :
+    forall m k v,
+      IM.find k m = Some v ->
+      (interp_state (@handle_mem_spec Effin _) (trigger (LoadE k) : ctree MemE Bspec nat) m) ~
+        (ret (m, v) : ctree Effin Bspec (memory * nat)%type).
+  Proof.
+    intros m k v LUP.
+    setoid_rewrite interp_state_trigger.
+    cbn.
+    rewrite LUP.
+    rewrite bind_ret_l.
+    apply sb_guard_l.
+    reflexivity.
+  Qed.
+
+  Ltac inj_pair2_existT :=
+    repeat
       match goal with
       | H : _ |- _ => apply Eqdep.EqdepTheory.inj_pair2 in H
       end.
 
-Ltac subst_existT :=
-  inj_pair2_existT; subst.
+  Ltac subst_existT :=
+    inj_pair2_existT; subst.
 
-(* #[global] Instance Reflexive_update_val_rel {E X} L R0 : *)
-(*   Reflexive L -> *)
-(*   Reflexive R0 -> *)
-(*   Reflexive (@update_val_rel E E X X L R0). *)
-(* Proof. *)
-(*   red. intros. destruct x. *)
-(*   1-2: constructor; eauto; intros VAL; inversion VAL. *)
-(*   assert (X = X0 \/ X <> X0) as [EQ | NEQ] by admit. *)
-(*   - subst. *)
-(*     apply update_Val. *)
-(*     reflexivity. *)
-(*   - constructor. *)
-(*     + intros VAL. *)
-(*       inv VAL. *)
-(*       subst_existT. *)
-(*     inv VAL. *)
-(* Qed. *)
+  (* #[global] Instance Reflexive_update_val_rel {E X} L R0 : *)
+  (*   Reflexive L -> *)
+  (*   Reflexive R0 -> *)
+  (*   Reflexive (@update_val_rel E E X X L R0). *)
+  (* Proof. *)
+  (*   red. intros. destruct x. *)
+  (*   1-2: constructor; eauto; intros VAL; inversion VAL. *)
+  (*   assert (X = X0 \/ X <> X0) as [EQ | NEQ] by admit. *)
+  (*   - subst. *)
+  (*     apply update_Val. *)
+  (*     reflexivity. *)
+  (*   - constructor. *)
+  (*     + intros VAL. *)
+  (*       inv VAL. *)
+  (*       subst_existT. *)
+  (*     inv VAL. *)
+  (* Qed. *)
 
-Lemma raise_bind :
-  forall E `{FailureE -< E} B R1 R2 R3 msg (k : R1 -> ctree E B R2),
-    ((raise msg : ctree E B R1) >>= k) ~ (raise msg : ctree E B R3).
-Proof.
-  intros E H B R1 R2 R3 msg k.
-  cbn.
-  unfold raise.
-  rewrite bind_bind.
-  apply sbisim_clo_bind with (R0:=eq).
-  - eapply Lequiv_sbisim; [| reflexivity].
-    symmetry.
-    apply update_val_rel_eq.
-  - intros [].
-Qed.
+  Lemma raise_bind :
+    forall E `{FailureE -< E} B R1 R2 R3 msg (k : R1 -> ctree E B R2),
+      ((raise msg : ctree E B R1) >>= k) ~ (raise msg : ctree E B R3).
+  Proof.
+    intros E H B R1 R2 R3 msg k.
+    cbn.
+    unfold raise.
+    rewrite bind_bind.
+    apply sbisim_clo_bind with (R0:=eq).
+    - eapply Lequiv_sbisim; [| reflexivity].
+      symmetry.
+      apply update_val_rel_eq.
+    - intros [].
+  Qed.
 
-Lemma store_fail_lemma :
-  forall m k v,
-    IM.mem k m = false ->
-    (interp_state handle_mem_spec (trigger (StoreE k v) : ctree MemE Bspec unit) m) ~
-      (raise "Store to unallocated address." : ctree Effin Bspec (memory * unit)%type).
-Proof.
-  intros m k v MEM.
-  setoid_rewrite interp_state_trigger.
-  cbn.
-  destruct (IM.find k m) eqn:LUP.
-  - exfalso.
-    apply IM.find_2 in LUP.
-    assert (IM.In k m) as IN.
-    exists n. apply LUP.
-    apply IM.mem_1 in IN.
-    rewrite MEM in IN; discriminate.
-  - rewrite raise_bind.
+  Lemma store_fail_lemma :
+    forall m k v,
+      IM.mem k m = false ->
+      (interp_state handle_mem_spec (trigger (StoreE k v) : ctree MemE Bspec unit) m) ~
+        (raise "Store to unallocated address." : ctree Effin Bspec (memory * unit)%type).
+  Proof.
+    intros m k v MEM.
+    setoid_rewrite interp_state_trigger.
+    cbn.
+    destruct (IM.find k m) eqn:LUP.
+    - exfalso.
+      apply IM.find_2 in LUP.
+      assert (IM.In k m) as IN.
+      exists n. apply LUP.
+      apply IM.mem_1 in IN.
+      rewrite MEM in IN; discriminate.
+    - rewrite raise_bind.
+      reflexivity.
+  Qed.
+
+  Lemma load_fails_lemma :
+    forall m k,
+      IM.mem k m = false ->
+      (interp_state handle_mem_spec (trigger (LoadE k) : ctree MemE Bspec nat) m) ~
+        (raise "Load from unallocated address." : ctree Effin Bspec (memory * unit)%type).
+  Proof.
+    intros m k MEM.
+    setoid_rewrite interp_state_trigger.
+    cbn.
+    destruct (IM.find k m) eqn:LUP.
+    - exfalso.
+      apply IM.find_2 in LUP.
+      assert (IM.In k m) as IN.
+      exists n. apply LUP.
+      apply IM.mem_1 in IN.
+      rewrite MEM in IN; discriminate.
+    - cbn.
+      (* Why can't I just rewrite? *)
+      pose proof (@raise_bind Effin _ Bspec (memory * nat)%type (memory * nat)%type (memory * unit)%type "Load from unallocated address." (fun x => Guard (Ret x))).
+      cbn in *.
+      apply H.
+  Qed.
+
+  Variant ForallE : Type -> Type :=
+    | Spec_forall A : ForallE A.
+
+  Definition forall_spec {E} (A : Type) : ctree E ForallE A :=
+    Br (Spec_forall A) (fun (a : A) => Ret a).
+
+  Lemma blah :
+    @ssim Effin Effin void1 ForallE nat nat eq
+      (ret 1) (forall_spec nat).
+  Proof.
+    unfold forall_spec.
+    apply ssim_br_r with (x:=1).
+    apply ssim_ret.
     reflexivity.
-Qed.
+  Qed.
 
-Lemma load_fails_lemma :
-  forall m k,
-    IM.mem k m = false ->
-    (interp_state handle_mem_spec (trigger (LoadE k) : ctree MemE Bspec nat) m) ~
-      (raise "Load from unallocated address." : ctree Effin Bspec (memory * unit)%type).
-Proof.
-  intros m k MEM.
-  setoid_rewrite interp_state_trigger.
-  cbn.
-  destruct (IM.find k m) eqn:LUP.
-  - exfalso.
-    apply IM.find_2 in LUP.
-    assert (IM.In k m) as IN.
-    exists n. apply LUP.
-    apply IM.mem_1 in IN.
-    rewrite MEM in IN; discriminate.
-  - cbn.
-    (* Why can't I just rewrite? *)
-    pose proof (@raise_bind Effin _ Bspec (memory * nat)%type (memory * nat)%type (memory * unit)%type "Load from unallocated address." (fun x => Guard (Ret x))).
-    cbn in *.
-    apply H.
-Qed.
-
-Variant ForallE : Type -> Type :=
-  | Spec_forall A : ForallE A.
-
-Definition forall_spec {E} (A : Type) : ctree E ForallE A :=
-  Br (Spec_forall A) (fun (a : A) => Ret a).
-
-Lemma blah :
-  @ssim Effin Effin void1 ForallE nat nat eq
-  (ret 1) (forall_spec nat).
-Proof.
-  unfold forall_spec.
-  apply ssim_br_r with (x:=1).
-  apply ssim_ret.
-  reflexivity.
-Qed.
-
-(* This doesn't work. The thing on the right is an empty set, and the
+  (* This doesn't work. The thing on the right is an empty set, and the
 refinement relation doesn't hold vacuously *)
-Lemma ub_test :
-  @ssim Effin Effin ForallE ForallE nat nat eq
-    (ret 1) (x <- forall_spec void;; ret 9).
-Proof.
-  unfold forall_spec.
-  cbn.
-  rewrite bind_br.
-  (* No way to instantiate x *)
-  Fail apply ssim_br_r.
-Abort.
+  Lemma ub_test :
+    @ssim Effin Effin ForallE ForallE nat nat eq
+      (ret 1) (x <- forall_spec void;; ret 9).
+  Proof.
+    unfold forall_spec.
+    cbn.
+    rewrite bind_br.
+    (* No way to instantiate x *)
+    Fail apply ssim_br_r.
+  Abort.
 
-(* This *does* work. The smaller set on the left is empty, and therefore a
+  (* This *does* work. The smaller set on the left is empty, and therefore a
    subset of the thing on the right. *)
-Lemma ub_test_l :
-  @ssim Effin Effin ForallE ForallE nat nat eq
-    (x <- forall_spec void;; ret 9) (ret 1).
-Proof.
-  unfold forall_spec.
-  cbn.
-  rewrite bind_br.
-  apply ssim_br_l.
-  intros [].
-Qed.
+  Lemma ub_test_l :
+    @ssim Effin Effin ForallE ForallE nat nat eq
+      (x <- forall_spec void;; ret 9) (ret 1).
+  Proof.
+    unfold forall_spec.
+    cbn.
+    rewrite bind_br.
+    apply ssim_br_l.
+    intros [].
+  Qed.
 
-Lemma blah' :
-  @ssim Effin Effin ForallE ForallE nat nat eq
-    (forall_spec nat)
-    (forall_spec nat).
-Proof.
-  unfold forall_spec.
-  apply ssim_br_id.
-  intros x.
-  apply ssim_ret; reflexivity.
-Qed.
+  Lemma blah' :
+    @ssim Effin Effin ForallE ForallE nat nat eq
+      (forall_spec nat)
+      (forall_spec nat).
+  Proof.
+    unfold forall_spec.
+    apply ssim_br_id.
+    intros x.
+    apply ssim_ret; reflexivity.
+  Qed.
 
-Lemma store_forward_with_rewrites' :
-  forall m v,
-    @ssim Effin Effin Bspec Bspec _ _ eq
-      (ret v)
-      (fmap snd (interp_state handle_mem_spec (store_prog v) m)).
-Proof.
-  intros m v.
-  unfold store_prog.
-  cbn.
-  repeat setoid_rewrite interp_state_bind.
-  repeat setoid_rewrite bind_bind.
+  Lemma store_forward_with_rewrites' :
+    forall m v,
+      @ssim Effin Effin Bspec Bspec _ _ eq
+        (ret v)
+        (fmap snd (interp_state handle_mem_spec (store_prog v) m)).
+  Proof.
+    intros m v.
+    unfold store_prog.
+    cbn.
+    repeat setoid_rewrite interp_state_bind.
+    repeat setoid_rewrite bind_bind.
 
-  rewrite <- alloc_lemma'; cbn.
-  rewrite bind_ret_l; cbn.
-  rewrite store_succ_lemma; cbn; eauto.
-  2: apply mem_add_eq.
+    rewrite <- alloc_lemma'; cbn.
+    rewrite bind_ret_l; cbn.
+    rewrite store_succ_lemma; cbn; eauto.
+    2: apply mem_add_eq.
 
-  rewrite bind_ret_l; cbn.
-  rewrite load_succ_lemma; [cbn; eauto | apply find_add_eq].
+    rewrite bind_ret_l; cbn.
+    rewrite load_succ_lemma; [cbn; eauto | apply find_add_eq].
 
-  rewrite bind_ret_l.
-  cbn.
-  reflexivity.
-Qed.
+    rewrite bind_ret_l.
+    cbn.
+    reflexivity.
+  Qed.
 
-Hint Rewrite
-  @bind_bind
-  @bind_branch
-  @bind_vis
-  @bind_ret_l
-  @interp_state_bind
-  @interp_state_trigger
-  alloc_lemma'
-  store_succ_lemma
-  load_succ_lemma : SolveMem.
+  Hint Rewrite
+    @bind_bind
+    @bind_branch
+    @bind_vis
+    @bind_ret_l
+    @interp_state_bind
+    @interp_state_trigger
+    alloc_lemma'
+    store_succ_lemma
+    load_succ_lemma : SolveMem.
 
-Hint Resolve
-  @bind_bind
-  @bind_vis
-  @bind_ret_l
-  @interp_state_bind
-  @interp_state_trigger
-  @ssim_br_r
-  @ssim_br_l
-  @ssim_guard_r
-  @ssim_guard_l
-  @ssim_ret
-  alloc_lemma'
-  store_succ_lemma
-  load_succ_lemma 
-  mem_add_eq
-  find_add_eq : SolveMem.
+  Hint Resolve
+    @bind_bind
+    @bind_vis
+    @bind_ret_l
+    @interp_state_bind
+    @interp_state_trigger
+    @ssim_br_r
+    @ssim_br_l
+    @ssim_guard_r
+    @ssim_guard_l
+    @ssim_ret
+    alloc_lemma'
+    store_succ_lemma
+    load_succ_lemma 
+    mem_add_eq
+    find_add_eq : SolveMem.
 
-Ltac solve_refines :=
-  cbn;
-  repeat setoid_rewrite interp_state_bind;
-  cbn;
-  repeat (autorewrite with SolveMem; cbn);
-  eauto with SolveMem.
+  Ltac solve_refines :=
+    cbn;
+    repeat setoid_rewrite interp_state_bind;
+    cbn;
+    repeat (autorewrite with SolveMem; cbn);
+    eauto with SolveMem.
 
-Lemma store_forward_with_rewrites'' :
-  forall m v,
-    @ssim Effin Effin Bspec Bspec _ _ eq
-      (ret v)
-      (fmap snd (interp_state handle_mem_spec (store_prog v) m)).
-Proof.
-  intros m v.
-  cbn.
-  unfold CTree.map.
-  unfold store_prog.
-  solve_refines.
-  unfold do_alloc.
-  rewrite bind_bind.
-  rewrite bind_branch.
-  eapply ssim_br_r.
-  cbn.
-  rewrite bind_ret_l.
-  rewrite bind_guard.
-  apply ssim_guard_r.
-  solve_refines.
-  Unshelve.
-  apply alloc_sigma.
-Qed.
+  Lemma store_forward_with_rewrites'' :
+    forall m v,
+      @ssim Effin Effin Bspec Bspec _ _ eq
+        (ret v)
+        (fmap snd (interp_state handle_mem_spec (store_prog v) m)).
+  Proof.
+    intros m v.
+    cbn.
+    unfold CTree.map.
+    unfold store_prog.
+    solve_refines.
+    unfold do_alloc.
+    rewrite bind_bind.
+    rewrite bind_branch.
+    eapply ssim_br_r.
+    cbn.
+    rewrite bind_ret_l.
+    rewrite bind_guard.
+    apply ssim_guard_r.
+    solve_refines.
+    Unshelve.
+    apply alloc_sigma.
+  Qed.
 
-Lemma store_forward_with_rewrites :
-  forall m v,
-    @ssim Effin Effin Bspec Bspec _ _ eq
-      (fmap snd (interp_state handle_mem_spec (store_prog v) m))
-      (ret v).
-Proof.
-  intros m v.
-  cbn.
-  unfold CTree.map.
-  cbn.
+  Lemma store_forward_with_rewrites :
+    forall m v,
+      @ssim Effin Effin Bspec Bspec _ _ eq
+        (fmap snd (interp_state handle_mem_spec (store_prog v) m))
+        (ret v).
+  Proof.
+    intros m v.
+    cbn.
+    unfold CTree.map.
+    cbn.
 
-  Opaque IM.mem IM.find IM.add.
-  setoid_rewrite interp_state_bind.
-  setoid_rewrite interp_state_bind.
-  cbn.
-  repeat setoid_rewrite bind_bind.
-  cbn.
+    Opaque IM.mem IM.find IM.add.
+    setoid_rewrite interp_state_bind.
+    setoid_rewrite interp_state_bind.
+    cbn.
+    repeat setoid_rewrite bind_bind.
+    cbn.
 
-  (* This first alloc is hard to rewrite :|
+    (* This first alloc is hard to rewrite :|
 
      alloc is generally not a refinement of a ret because it can
      return many values. The overall lemma holds, however, because
      this detail is hidden from the outside.
-   *)
-  setoid_rewrite interp_state_trigger at 1.
-  cbn.
-  unfold do_alloc.
-  repeat rewrite bind_bind.
-  rewrite bind_branch.
-  apply ssim_br_l.
-  intros [k m'].
-  solve_refines.
-  rewrite bind_guard.
-  apply ssim_guard_l.
-  solve_refines.
-Qed.
+     *)
+    setoid_rewrite interp_state_trigger at 1.
+    cbn.
+    unfold do_alloc.
+    repeat rewrite bind_bind.
+    rewrite bind_branch.
+    apply ssim_br_l.
+    intros [k m'].
+    solve_refines.
+    rewrite bind_guard.
+    apply ssim_guard_l.
+    solve_refines.
+  Qed.
 
 
-(* (* May need complete simulations to break this proof up like this... May be resolved in askrcv ctrees branch *) *)
-(* Lemma store_forward_stronger : *)
-(*   forall m v, *)
-(*     (ret v : ctree Effin Bspec nat) ~ *)
-(*       (fmap snd (interp_state (@handle_mem_spec Effin _) (store_prog v) m)). *)
-(* Proof. *)
-(*   intros m v. *)
-(*   sbisim *)
-(*   rewrite store_forward_with_rewrites'. *)
-(*   split. *)
-(*   apply store_forward_with_rewrites. *)
-(*   apply store_forward_with_rewrites'. *)
-(* Qed. *)
+  (* (* May need complete simulations to break this proof up like this... May be resolved in askrcv ctrees branch *) *)
+  (* Lemma store_forward_stronger : *)
+  (*   forall m v, *)
+  (*     (ret v : ctree Effin Bspec nat) ~ *)
+  (*       (fmap snd (interp_state (@handle_mem_spec Effin _) (store_prog v) m)). *)
+  (* Proof. *)
+  (*   intros m v. *)
+  (*   sbisim *)
+  (*   rewrite store_forward_with_rewrites'. *)
+  (*   split. *)
+  (*   apply store_forward_with_rewrites. *)
+  (*   apply store_forward_with_rewrites'. *)
+  (* Qed. *)
+End Memory.
